Correct dist_prod_coprod2 and dist_prod_coprod_inv2 types

ETCS_Coproduct.thy
@@ -1775,110 +1775,110 @@ qed
 
 
 definition dist_prod_coprod2 :: "cset \<Rightarrow> cset \<Rightarrow> cset \<Rightarrow> cfunc" where
-  "dist_prod_coprod2 A B C = swap A (B \<Coprod> C) \<circ>\<^sub>c dist_prod_coprod A B C \<circ>\<^sub>c (swap B A \<bowtie>\<^sub>f swap C A)"
+  "dist_prod_coprod2 A B C = swap C (A \<Coprod> B) \<circ>\<^sub>c dist_prod_coprod C A B \<circ>\<^sub>c (swap A C \<bowtie>\<^sub>f swap B C)"
 
 lemma dist_prod_coprod2_type[type_rule]:
-  "dist_prod_coprod2 A B C : (B \<times>\<^sub>c A) \<Coprod> (C \<times>\<^sub>c A) \<rightarrow> (B \<Coprod> C) \<times>\<^sub>c A"
+  "dist_prod_coprod2 A B C : (A \<times>\<^sub>c C) \<Coprod> (B \<times>\<^sub>c C) \<rightarrow> (A \<Coprod> B) \<times>\<^sub>c C"
   unfolding dist_prod_coprod2_def by typecheck_cfuncs
 
 lemma dist_prod_coprod2_left_ap:
-  assumes "a \<in>\<^sub>c A" "b \<in>\<^sub>c B"
-  shows "dist_prod_coprod2 A B C \<circ>\<^sub>c (left_coproj (B \<times>\<^sub>c A) (C \<times>\<^sub>c A) \<circ>\<^sub>c \<langle>b, a\<rangle>) = \<langle>left_coproj B C \<circ>\<^sub>c b, a\<rangle>"
+  assumes "a \<in>\<^sub>c A" "c \<in>\<^sub>c C"
+  shows "dist_prod_coprod2 A B C \<circ>\<^sub>c (left_coproj (A \<times>\<^sub>c C) (B \<times>\<^sub>c C) \<circ>\<^sub>c \<langle>a, c\<rangle>) = \<langle>left_coproj A B \<circ>\<^sub>c a, c\<rangle>"
 proof -
-  have "dist_prod_coprod2 A B C \<circ>\<^sub>c (left_coproj (B \<times>\<^sub>c A) (C \<times>\<^sub>c A) \<circ>\<^sub>c \<langle>b, a\<rangle>)
-    = (swap A (B \<Coprod> C) \<circ>\<^sub>c dist_prod_coprod A B C \<circ>\<^sub>c (swap B A \<bowtie>\<^sub>f swap C A)) \<circ>\<^sub>c (left_coproj (B \<times>\<^sub>c A) (C \<times>\<^sub>c A) \<circ>\<^sub>c \<langle>b, a\<rangle>)"
+  have "dist_prod_coprod2 A B C \<circ>\<^sub>c (left_coproj (A \<times>\<^sub>c C) (B \<times>\<^sub>c C) \<circ>\<^sub>c \<langle>a, c\<rangle>)
+    = (swap C (A \<Coprod> B) \<circ>\<^sub>c dist_prod_coprod C A B \<circ>\<^sub>c (swap A C \<bowtie>\<^sub>f swap B C)) \<circ>\<^sub>c (left_coproj (A \<times>\<^sub>c C) (B \<times>\<^sub>c C) \<circ>\<^sub>c \<langle>a, c\<rangle>)"
     unfolding dist_prod_coprod2_def by auto
-  also have "... = swap A (B \<Coprod> C) \<circ>\<^sub>c dist_prod_coprod A B C \<circ>\<^sub>c ((swap B A \<bowtie>\<^sub>f swap C A) \<circ>\<^sub>c left_coproj (B \<times>\<^sub>c A) (C \<times>\<^sub>c A)) \<circ>\<^sub>c \<langle>b, a\<rangle>"
+  also have "... = swap C (A \<Coprod> B) \<circ>\<^sub>c dist_prod_coprod C A B \<circ>\<^sub>c ((swap A C \<bowtie>\<^sub>f swap B C) \<circ>\<^sub>c left_coproj (A \<times>\<^sub>c C) (B \<times>\<^sub>c C)) \<circ>\<^sub>c \<langle>a, c\<rangle>"
     using assms by (typecheck_cfuncs, smt comp_associative2)
-  also have "... = swap A (B \<Coprod> C) \<circ>\<^sub>c dist_prod_coprod A B C \<circ>\<^sub>c (left_coproj (A \<times>\<^sub>c B) (A \<times>\<^sub>c C) \<circ>\<^sub>c swap B A) \<circ>\<^sub>c \<langle>b, a\<rangle>"
+  also have "... = swap C (A \<Coprod> B) \<circ>\<^sub>c dist_prod_coprod C A B \<circ>\<^sub>c (left_coproj (C \<times>\<^sub>c A) (C \<times>\<^sub>c B) \<circ>\<^sub>c swap A C) \<circ>\<^sub>c \<langle>a, c\<rangle>"
     using assms by (typecheck_cfuncs, auto simp add: left_coproj_cfunc_bowtie_prod)
-  also have "... = swap A (B \<Coprod> C) \<circ>\<^sub>c dist_prod_coprod A B C \<circ>\<^sub>c left_coproj (A \<times>\<^sub>c B) (A \<times>\<^sub>c C) \<circ>\<^sub>c swap B A \<circ>\<^sub>c \<langle>b, a\<rangle>"
+  also have "... = swap C (A \<Coprod> B) \<circ>\<^sub>c dist_prod_coprod C A B \<circ>\<^sub>c left_coproj (C \<times>\<^sub>c A) (C \<times>\<^sub>c B) \<circ>\<^sub>c swap A C \<circ>\<^sub>c \<langle>a, c\<rangle>"
     using assms by (typecheck_cfuncs, auto simp add: comp_associative2)
-  also have "... = swap A (B \<Coprod> C) \<circ>\<^sub>c dist_prod_coprod A B C \<circ>\<^sub>c left_coproj (A \<times>\<^sub>c B) (A \<times>\<^sub>c C) \<circ>\<^sub>c \<langle>a, b\<rangle>"
+  also have "... = swap C (A \<Coprod> B) \<circ>\<^sub>c dist_prod_coprod C A B \<circ>\<^sub>c left_coproj (C \<times>\<^sub>c A) (C \<times>\<^sub>c B) \<circ>\<^sub>c \<langle>c, a\<rangle>"
     using assms swap_ap by (typecheck_cfuncs, auto)
-  also have "... = swap A (B \<Coprod> C) \<circ>\<^sub>c \<langle>a, left_coproj B C \<circ>\<^sub>c b\<rangle>"
+  also have "... = swap C (A \<Coprod> B) \<circ>\<^sub>c \<langle>c, left_coproj A B \<circ>\<^sub>c a\<rangle>"
     using assms by (typecheck_cfuncs, simp add: dist_prod_coprod_left_ap)
-  also have "... = \<langle>left_coproj B C \<circ>\<^sub>c b, a\<rangle>"
+  also have "... = \<langle>left_coproj A B \<circ>\<^sub>c a, c\<rangle>"
     using assms swap_ap by (typecheck_cfuncs, auto)
   then show ?thesis
     using calculation by auto
 qed
 
 lemma dist_prod_coprod2_right_ap:
-  assumes "a \<in>\<^sub>c A" "c \<in>\<^sub>c C"
-  shows "dist_prod_coprod2 A B C \<circ>\<^sub>c (right_coproj (B \<times>\<^sub>c A) (C \<times>\<^sub>c A) \<circ>\<^sub>c \<langle>c, a\<rangle>) = \<langle>right_coproj B C \<circ>\<^sub>c c, a\<rangle>"
+  assumes "b \<in>\<^sub>c B" "c \<in>\<^sub>c C"
+  shows "dist_prod_coprod2 A B C \<circ>\<^sub>c (right_coproj (A \<times>\<^sub>c C) (B \<times>\<^sub>c C) \<circ>\<^sub>c \<langle>b, c\<rangle>) = \<langle>right_coproj A B \<circ>\<^sub>c b, c\<rangle>"
 proof -
-  have "dist_prod_coprod2 A B C \<circ>\<^sub>c (right_coproj (B \<times>\<^sub>c A) (C \<times>\<^sub>c A) \<circ>\<^sub>c \<langle>c, a\<rangle>)
-    = (swap A (B \<Coprod> C) \<circ>\<^sub>c dist_prod_coprod A B C \<circ>\<^sub>c (swap B A \<bowtie>\<^sub>f swap C A)) \<circ>\<^sub>c (right_coproj (B \<times>\<^sub>c A) (C \<times>\<^sub>c A) \<circ>\<^sub>c \<langle>c, a\<rangle>)"
+  have "dist_prod_coprod2 A B C \<circ>\<^sub>c (right_coproj (A \<times>\<^sub>c C) (B \<times>\<^sub>c C) \<circ>\<^sub>c \<langle>b, c\<rangle>)
+    = (swap C (A \<Coprod> B) \<circ>\<^sub>c dist_prod_coprod C A B \<circ>\<^sub>c (swap A C \<bowtie>\<^sub>f swap B C)) \<circ>\<^sub>c (right_coproj (A \<times>\<^sub>c C) (B \<times>\<^sub>c C) \<circ>\<^sub>c \<langle>b, c\<rangle>)"
     unfolding dist_prod_coprod2_def by auto
-  also have "... = swap A (B \<Coprod> C) \<circ>\<^sub>c dist_prod_coprod A B C \<circ>\<^sub>c ((swap B A \<bowtie>\<^sub>f swap C A) \<circ>\<^sub>c right_coproj (B \<times>\<^sub>c A) (C \<times>\<^sub>c A)) \<circ>\<^sub>c \<langle>c, a\<rangle>"
+  also have "... = swap C (A \<Coprod> B) \<circ>\<^sub>c dist_prod_coprod C A B \<circ>\<^sub>c ((swap A C \<bowtie>\<^sub>f swap B C) \<circ>\<^sub>c right_coproj (A \<times>\<^sub>c C) (B \<times>\<^sub>c C)) \<circ>\<^sub>c \<langle>b, c\<rangle>"
     using assms by (typecheck_cfuncs, smt comp_associative2)
-  also have "... = swap A (B \<Coprod> C) \<circ>\<^sub>c dist_prod_coprod A B C \<circ>\<^sub>c (right_coproj (A \<times>\<^sub>c B) (A \<times>\<^sub>c C) \<circ>\<^sub>c swap C A) \<circ>\<^sub>c \<langle>c, a\<rangle>"
+  also have "... = swap C (A \<Coprod> B) \<circ>\<^sub>c dist_prod_coprod C A B \<circ>\<^sub>c (right_coproj (C \<times>\<^sub>c A) (C \<times>\<^sub>c B) \<circ>\<^sub>c swap B C) \<circ>\<^sub>c \<langle>b, c\<rangle>"
     using assms by (typecheck_cfuncs, auto simp add: right_coproj_cfunc_bowtie_prod)
-  also have "... = swap A (B \<Coprod> C) \<circ>\<^sub>c dist_prod_coprod A B C \<circ>\<^sub>c right_coproj (A \<times>\<^sub>c B) (A \<times>\<^sub>c C) \<circ>\<^sub>c swap C A \<circ>\<^sub>c \<langle>c, a\<rangle>"
+  also have "... = swap C (A \<Coprod> B) \<circ>\<^sub>c dist_prod_coprod C A B \<circ>\<^sub>c right_coproj (C \<times>\<^sub>c A) (C \<times>\<^sub>c B) \<circ>\<^sub>c swap B C \<circ>\<^sub>c \<langle>b, c\<rangle>"
     using assms by (typecheck_cfuncs, auto simp add: comp_associative2)
-  also have "... = swap A (B \<Coprod> C) \<circ>\<^sub>c dist_prod_coprod A B C \<circ>\<^sub>c right_coproj (A \<times>\<^sub>c B) (A \<times>\<^sub>c C) \<circ>\<^sub>c \<langle>a, c\<rangle>"
+  also have "... = swap C (A \<Coprod> B) \<circ>\<^sub>c dist_prod_coprod C A B \<circ>\<^sub>c right_coproj (C \<times>\<^sub>c A) (C \<times>\<^sub>c B) \<circ>\<^sub>c \<langle>c, b\<rangle>"
     using assms swap_ap by (typecheck_cfuncs, auto)
-  also have "... = swap A (B \<Coprod> C) \<circ>\<^sub>c \<langle>a, right_coproj B C \<circ>\<^sub>c c\<rangle>"
+  also have "... = swap C (A \<Coprod> B) \<circ>\<^sub>c \<langle>c, right_coproj A B \<circ>\<^sub>c b\<rangle>"
     using assms by (typecheck_cfuncs, simp add: dist_prod_coprod_right_ap)
-  also have "... = \<langle>right_coproj B C \<circ>\<^sub>c c, a\<rangle>"
+  also have "... = \<langle>right_coproj A B \<circ>\<^sub>c b, c\<rangle>"
     using assms swap_ap by (typecheck_cfuncs, auto)
   then show ?thesis
     using calculation by auto
 qed
 
 definition dist_prod_coprod_inv2 :: "cset \<Rightarrow> cset \<Rightarrow> cset \<Rightarrow> cfunc" where
-  "dist_prod_coprod_inv2 A B C = (swap A B \<bowtie>\<^sub>f swap A C) \<circ>\<^sub>c dist_prod_coprod_inv A B C \<circ>\<^sub>c swap (B \<Coprod> C) A"
+  "dist_prod_coprod_inv2 A B C = (swap C A \<bowtie>\<^sub>f swap C B) \<circ>\<^sub>c dist_prod_coprod_inv C A B \<circ>\<^sub>c swap (A \<Coprod> B) C"
 
 lemma dist_prod_coprod_inv2_type[type_rule]:
-  "dist_prod_coprod_inv2 A B C : (B \<Coprod> C) \<times>\<^sub>c A \<rightarrow> (B \<times>\<^sub>c A) \<Coprod> (C \<times>\<^sub>c A)"
+  "dist_prod_coprod_inv2 A B C : (A \<Coprod> B) \<times>\<^sub>c C \<rightarrow> (A \<times>\<^sub>c C) \<Coprod> (B \<times>\<^sub>c C)"
   unfolding dist_prod_coprod_inv2_def by typecheck_cfuncs
 
 lemma dist_prod_coprod_inv2_left_ap:
-  assumes "a \<in>\<^sub>c A" "b \<in>\<^sub>c B"
-  shows "dist_prod_coprod_inv2 A B C \<circ>\<^sub>c \<langle>left_coproj B C \<circ>\<^sub>c b, a\<rangle> = left_coproj (B \<times>\<^sub>c A) (C \<times>\<^sub>c A) \<circ>\<^sub>c \<langle>b, a\<rangle>"
+  assumes "a \<in>\<^sub>c A" "c \<in>\<^sub>c C"
+  shows "dist_prod_coprod_inv2 A B C \<circ>\<^sub>c \<langle>left_coproj A B \<circ>\<^sub>c a, c\<rangle> = left_coproj (A \<times>\<^sub>c C) (B \<times>\<^sub>c C) \<circ>\<^sub>c \<langle>a, c\<rangle>"
 proof -
-  have "dist_prod_coprod_inv2 A B C \<circ>\<^sub>c \<langle>left_coproj B C \<circ>\<^sub>c b, a\<rangle>
-    = ((swap A B \<bowtie>\<^sub>f swap A C) \<circ>\<^sub>c dist_prod_coprod_inv A B C \<circ>\<^sub>c swap (B \<Coprod> C) A) \<circ>\<^sub>c \<langle>left_coproj B C \<circ>\<^sub>c b, a\<rangle>"
+  have "dist_prod_coprod_inv2 A B C \<circ>\<^sub>c \<langle>left_coproj A B \<circ>\<^sub>c a, c\<rangle>
+    = ((swap C A \<bowtie>\<^sub>f swap C B) \<circ>\<^sub>c dist_prod_coprod_inv C A B \<circ>\<^sub>c swap (A \<Coprod> B) C) \<circ>\<^sub>c \<langle>left_coproj A B \<circ>\<^sub>c a, c\<rangle>"
     unfolding dist_prod_coprod_inv2_def by auto
-  also have "... = (swap A B \<bowtie>\<^sub>f swap A C) \<circ>\<^sub>c dist_prod_coprod_inv A B C \<circ>\<^sub>c swap (B \<Coprod> C) A \<circ>\<^sub>c \<langle>left_coproj B C \<circ>\<^sub>c b, a\<rangle>"
+  also have "... = (swap C A \<bowtie>\<^sub>f swap C B) \<circ>\<^sub>c dist_prod_coprod_inv C A B \<circ>\<^sub>c swap (A \<Coprod> B) C \<circ>\<^sub>c \<langle>left_coproj A B \<circ>\<^sub>c a, c\<rangle>"
     using assms by (typecheck_cfuncs, smt comp_associative2)
-  also have "... = (swap A B \<bowtie>\<^sub>f swap A C) \<circ>\<^sub>c dist_prod_coprod_inv A B C \<circ>\<^sub>c \<langle>a, left_coproj B C \<circ>\<^sub>c b\<rangle>"
+  also have "... = (swap C A \<bowtie>\<^sub>f swap C B) \<circ>\<^sub>c dist_prod_coprod_inv C A B \<circ>\<^sub>c \<langle>c, left_coproj A B \<circ>\<^sub>c a\<rangle>"
     using assms swap_ap by (typecheck_cfuncs, auto)
-  also have "... = (swap A B \<bowtie>\<^sub>f swap A C) \<circ>\<^sub>c left_coproj (A \<times>\<^sub>c B) (A \<times>\<^sub>c C) \<circ>\<^sub>c \<langle>a, b\<rangle>"
+  also have "... = (swap C A \<bowtie>\<^sub>f swap C B) \<circ>\<^sub>c left_coproj (C \<times>\<^sub>c A) (C \<times>\<^sub>c B) \<circ>\<^sub>c \<langle>c, a\<rangle>"
     using assms by (typecheck_cfuncs, simp add: dist_prod_coprod_inv_left_ap)
-  also have "... = ((swap A B \<bowtie>\<^sub>f swap A C) \<circ>\<^sub>c left_coproj (A \<times>\<^sub>c B) (A \<times>\<^sub>c C)) \<circ>\<^sub>c \<langle>a, b\<rangle>"
+  also have "... = ((swap C A \<bowtie>\<^sub>f swap C B) \<circ>\<^sub>c left_coproj (C \<times>\<^sub>c A) (C \<times>\<^sub>c B)) \<circ>\<^sub>c \<langle>c, a\<rangle>"
     using assms by (typecheck_cfuncs, smt comp_associative2)
-  also have "... = (left_coproj (B \<times>\<^sub>c A) (C \<times>\<^sub>c A) \<circ>\<^sub>c swap A B) \<circ>\<^sub>c \<langle>a, b\<rangle>"
+  also have "... = (left_coproj (A \<times>\<^sub>c C) (B \<times>\<^sub>c C) \<circ>\<^sub>c swap C A) \<circ>\<^sub>c \<langle>c, a\<rangle>"
     using assms left_coproj_cfunc_bowtie_prod by (typecheck_cfuncs, auto)
-  also have "... = left_coproj (B \<times>\<^sub>c A) (C \<times>\<^sub>c A) \<circ>\<^sub>c swap A B \<circ>\<^sub>c \<langle>a, b\<rangle>"
+  also have "... = left_coproj (A \<times>\<^sub>c C) (B \<times>\<^sub>c C) \<circ>\<^sub>c swap C A \<circ>\<^sub>c \<langle>c, a\<rangle>"
     using assms by (typecheck_cfuncs, smt comp_associative2)
-  also have "... = left_coproj (B \<times>\<^sub>c A) (C \<times>\<^sub>c A) \<circ>\<^sub>c \<langle>b, a\<rangle>"
+  also have "... = left_coproj (A \<times>\<^sub>c C) (B \<times>\<^sub>c C) \<circ>\<^sub>c \<langle>a, c\<rangle>"
     using assms swap_ap by (typecheck_cfuncs, auto)
   then show ?thesis
     using calculation by auto
 qed
 
 lemma dist_prod_coprod_inv2_right_ap:
-  assumes "a \<in>\<^sub>c A" "c \<in>\<^sub>c C"
-  shows "dist_prod_coprod_inv2 A B C \<circ>\<^sub>c \<langle>right_coproj B C \<circ>\<^sub>c c, a\<rangle> = right_coproj (B \<times>\<^sub>c A) (C \<times>\<^sub>c A) \<circ>\<^sub>c \<langle>c, a\<rangle>"
+  assumes "b \<in>\<^sub>c B" "c \<in>\<^sub>c C"
+  shows "dist_prod_coprod_inv2 A B C \<circ>\<^sub>c \<langle>right_coproj A B \<circ>\<^sub>c b, c\<rangle> = right_coproj (A \<times>\<^sub>c C) (B \<times>\<^sub>c C) \<circ>\<^sub>c \<langle>b, c\<rangle>"
 proof -
-  have "dist_prod_coprod_inv2 A B C \<circ>\<^sub>c \<langle>right_coproj B C \<circ>\<^sub>c c, a\<rangle>
-    = ((swap A B \<bowtie>\<^sub>f swap A C) \<circ>\<^sub>c dist_prod_coprod_inv A B C \<circ>\<^sub>c swap (B \<Coprod> C) A) \<circ>\<^sub>c \<langle>right_coproj B C \<circ>\<^sub>c c, a\<rangle>"
+  have "dist_prod_coprod_inv2 A B C \<circ>\<^sub>c \<langle>right_coproj A B \<circ>\<^sub>c b, c\<rangle>
+    = ((swap C A \<bowtie>\<^sub>f swap C B) \<circ>\<^sub>c dist_prod_coprod_inv C A B \<circ>\<^sub>c swap (A \<Coprod> B) C) \<circ>\<^sub>c \<langle>right_coproj A B \<circ>\<^sub>c b, c\<rangle>"
     unfolding dist_prod_coprod_inv2_def by auto
-  also have "... = (swap A B \<bowtie>\<^sub>f swap A C) \<circ>\<^sub>c dist_prod_coprod_inv A B C \<circ>\<^sub>c swap (B \<Coprod> C) A \<circ>\<^sub>c \<langle>right_coproj B C \<circ>\<^sub>c c, a\<rangle>"
+  also have "... = (swap C A \<bowtie>\<^sub>f swap C B) \<circ>\<^sub>c dist_prod_coprod_inv C A B \<circ>\<^sub>c swap (A \<Coprod> B) C \<circ>\<^sub>c \<langle>right_coproj A B \<circ>\<^sub>c b, c\<rangle>"
     using assms by (typecheck_cfuncs, smt comp_associative2)
-  also have "... = (swap A B \<bowtie>\<^sub>f swap A C) \<circ>\<^sub>c dist_prod_coprod_inv A B C \<circ>\<^sub>c \<langle>a, right_coproj B C \<circ>\<^sub>c c\<rangle>"
+  also have "... = (swap C A \<bowtie>\<^sub>f swap C B) \<circ>\<^sub>c dist_prod_coprod_inv C A B \<circ>\<^sub>c \<langle>c, right_coproj A B \<circ>\<^sub>c b\<rangle>"
     using assms swap_ap by (typecheck_cfuncs, auto)
-  also have "... = (swap A B \<bowtie>\<^sub>f swap A C) \<circ>\<^sub>c right_coproj (A \<times>\<^sub>c B) (A \<times>\<^sub>c C) \<circ>\<^sub>c \<langle>a, c\<rangle>"
+  also have "... = (swap C A \<bowtie>\<^sub>f swap C B) \<circ>\<^sub>c right_coproj (C \<times>\<^sub>c A) (C \<times>\<^sub>c B) \<circ>\<^sub>c \<langle>c, b\<rangle>"
     using assms by (typecheck_cfuncs, simp add: dist_prod_coprod_inv_right_ap)
-  also have "... = ((swap A B \<bowtie>\<^sub>f swap A C) \<circ>\<^sub>c right_coproj (A \<times>\<^sub>c B) (A \<times>\<^sub>c C)) \<circ>\<^sub>c \<langle>a, c\<rangle>"
+  also have "... = ((swap C A \<bowtie>\<^sub>f swap C B) \<circ>\<^sub>c right_coproj (C \<times>\<^sub>c A) (C \<times>\<^sub>c B)) \<circ>\<^sub>c \<langle>c, b\<rangle>"
     using assms by (typecheck_cfuncs, auto simp add: comp_associative2)
-  also have "... = (right_coproj (B \<times>\<^sub>c A) (C \<times>\<^sub>c A) \<circ>\<^sub>c swap A C) \<circ>\<^sub>c \<langle>a, c\<rangle>"
+  also have "... = (right_coproj (A \<times>\<^sub>c C) (B \<times>\<^sub>c C) \<circ>\<^sub>c swap C B) \<circ>\<^sub>c \<langle>c, b\<rangle>"
     using assms by (typecheck_cfuncs, auto simp add: right_coproj_cfunc_bowtie_prod)
-  also have "... = right_coproj (B \<times>\<^sub>c A) (C \<times>\<^sub>c A) \<circ>\<^sub>c swap A C \<circ>\<^sub>c \<langle>a, c\<rangle>"
+  also have "... = right_coproj (A \<times>\<^sub>c C) (B \<times>\<^sub>c C) \<circ>\<^sub>c swap C B \<circ>\<^sub>c \<langle>c, b\<rangle>"
     using assms by (typecheck_cfuncs, auto simp add: comp_associative2)
-  also have "... = right_coproj (B \<times>\<^sub>c A) (C \<times>\<^sub>c A) \<circ>\<^sub>c \<langle>c, a\<rangle>"
+  also have "... = right_coproj (A \<times>\<^sub>c C) (B \<times>\<^sub>c C) \<circ>\<^sub>c \<langle>b, c\<rangle>"
     using assms swap_ap by (typecheck_cfuncs, auto)
   then show ?thesis
     using calculation by auto
